specification/Lang.v
@@ -1,0 +1,49 @@
+Require Import String List.
+Import ListNotations.
+
+Inductive tm : Type :=
+| tm_var : string -> tm
+| tm_val : nat -> tm
+| tm_bin : tm -> tm -> tm
+| tm_un : tm -> tm
+| tm_let : string -> tm -> tm -> tm.
+
+Inductive ty : Type :=
+| Pub : ty
+| Sec : ty.
+
+Fixpoint subst (x : string) (s : nat) (t : tm) : tm :=
+  match t with
+  | tm_var y => if String.eqb x y then tm_val s else t
+  | tm_val _ => t 
+  | tm_bin t1 t2 => tm_bin (subst x s t1) (subst x s t2)
+  | tm_un t1 => tm_un (subst x s t1)
+  | tm_let x_b e b =>
+      let body := if String.eqb x x_b then b else (subst x s b) in
+      tm_let x_b (subst x s e) body
+  end.
+
+Definition smap : Type := list (string * nat).
+
+Fixpoint subst_many (bindings : smap) (t : tm) : tm :=
+  match bindings with
+  | [] => t
+  | (x, e) :: rest =>
+      let t' := subst x e t in
+      subst_many rest t'
+  end.
+
+Definition update {A} (Gamma : list (string * A)) (x : string) (t : A) : list (string * A) :=
+  (x, t) :: Gamma.
+
+
+Fixpoint lookup {A} (m : list (string * A)) (x : string) : option A :=
+  match m with
+  | [] => None
+  | (y, t) :: m' =>
+      if String.eqb x y then Some t
+      else lookup m' x
+  end.
+
+  
+  
